@prefix : <https://schema.org/> .
@prefix rdf: <http://www.w3.org/1999/02/22-rdf-syntax-ns#> .
@prefix rdfs: <http://www.w3.org/2000/01/rdf-schema#> .
@prefix owl: <http://www.w3.org/2002/07/owl#> .
@prefix xml: <http://www.w3.org/XML/1998/namespace> .
@prefix xsd: <http://www.w3.org/2001/XMLSchema#> .
@prefix stype: <https://w3id.org/software-types#> .

# This is an extension for schema.org for linking SoftwareSourceCode, SoftwareApplication and services like WebAPI
# all of the following are newly proposed as part of https://github.com/codemeta/codemeta/issues/271
# and are eventually proposed upstream to schema.org (but that may take a while)

#metadata
<https://w3id.org/software-types> rdf:type owl:Ontology ;
                            owl:versionIRI <https://w3id.org/software-types/1.0.0> ;
                            <http://purl.org/dc/terms/abstract> "This profile describes vocabulary terms needed to describe the metadata of software application types (e.g., command line, desktop, software package, software library, etc.)"@en ;
                            <http://purl.org/dc/elements/1.1/description> "This profile describes vocabulary terms needed to describe the metadata of software application types (e.g., command line, desktop, software package, software library, etc.)"@en ;
                            <http://purl.org/dc/elements/1.1/title> "The Software Types ontology"@en ;
                            <http://purl.org/dc/terms/created> "February 3rd, 2022"@en ;
                            <http://purl.org/dc/terms/creator> "Maarten van Gompel"@en ,
                                                               "Daniel Garijo"@en ;
                            <http://purl.org/dc/terms/license> <http://creativecommons.org/licenses/by/2.0/> ;
                            <http://purl.org/vocab/vann/preferredNamespacePrefix> "stype"@en ;
                            <http://purl.org/vocab/vann/preferredNamespaceUri> "https://w3id.org/software-types" ;
                            <http://schema.org/citation> "Cite this vocabulary as: van Gompel, M and Garijo, D. The Software Types ontology 1.0.0."@en ;
                            rdfs:comment "This profile describes vocabulary terms needed to describe the metadata of software application types (e.g., command line, desktop, software package, software library, etc.)"@en ;
                            owl:versionInfo "1.0.0"@en .

stype:CommandLineApplication a rdfs:Class ;
    rdfs:label "Command-Line Application" ;
    :source <https://github.com/codemeta/codemeta/issues/271> ;
    rdfs:comment "A software application offering a command-line interface." ;
    rdfs:subClassOf :SoftwareApplication .

stype:DesktopApplication a rdfs:Class ;
    rdfs:label "Desktop Application" ;
    :source <https://github.com/codemeta/codemeta/issues/271> ;
    rdfs:comment "A software application offering a graphical user interface on the deskop." ;
    rdfs:subClassOf :SoftwareApplication .

stype:TerminalApplication a rdfs:Class ;
    rdfs:label "Terminal Application" ;
    :source <https://github.com/codemeta/codemeta/issues/271> ;
    rdfs:comment "A software application offering a terminal text-based user interface (e.g. ncurses)." ;
    rdfs:subClassOf :SoftwareApplication .

stype:ServerApplication a rdfs:Class ;
    rdfs:label "Server Application" ;
    :source <https://github.com/codemeta/codemeta/issues/271> ;
    rdfs:comment "A software application running as a daemon providing a service, either locally or over a network, running in the background." ;
    rdfs:subClassOf :SoftwareApplication .

stype:SoftwareLibrary a rdfs:Class ;
    rdfs:label "Software Library" ;
    :source <https://github.com/codemeta/codemeta/issues/271> ;
    rdfs:comment "A software application offering an Application Programming Interface (API) for developers" ;
    rdfs:subClassOf :SoftwareApplication .

stype:SoftwareImage a rdfs:Class ;
    rdfs:label "Software Image" ;
    :source <https://github.com/codemeta/codemeta/issues/271> ;
    rdfs:comment "A software application in the form of an image (such as a container image or virtual machine image), distributes the application along with its wider dependency context." ;
    rdfs:subClassOf :SoftwareApplication .

stype:SoftwarePackage a rdfs:Class ;
    rdfs:label "Software Package" ;
    :source <https://github.com/codemeta/codemeta/issues/271> ;
    rdfs:comment "A software application in the form of a package for any particular package manager, distributes the application but not its wider dependency context." ;
    rdfs:subClassOf :SoftwareApplication .

stype:NotebookApplication a rdfs:Class ;
    rdfs:label "Notebook Application" ;
    :source <https://github.com/codemeta/codemeta/issues/271> ;
    rdfs:comment "A web application in the form of a notebook (e.g. Jupyter Notebook, R Notebook) or data story." ;
    rdfs:subClassOf :WebApplication .

# new properties:

stype:executableName a rdf:Property ;
    rdfs:label "executableName" ;
    :domainIncludes :SoftwareApplication , :SoftwareSourceCode ;
    :rangeIncludes :Text ;
    :source <https://github.com/codemeta/codemeta/issues/271> ;
    rdfs:comment: "Filename of the executable for the software application" .

# the following already exist, but are extended:

:targetProduct a rdf:Property ;
    rdfs:label "targetProduct" ;
    :domainIncludes :SoftwareSourceCode ;
    :rangeIncludes :SoftwareApplication , :WebAPI ;
    :source <https://github.com/codemeta/codemeta/issues/271> ;
    rdfs:comment "Product which is provided by the source code." .

:hasSourceCode a rdf:Property ;
    rdfs:label "hasSourceCode" ;
    :domainIncludes :SoftwareApplication , :WebAPI ;
    :rangeIncludes :SoftwareSourceCode ;
    :source <https://github.com/schemaorg/schemaorg/issues/1032>
    rdfs:comment "Source code of the software" .

:WebApplication a rdfs:Class ;
    rdfs:subClassOf stype:ServerApplication .

# copied unchanged from earlier proposals:

:WebAPI a rdfs:Class ;
    rdfs:label "WebAPI" ;
    :isPartOf <https://pending.schema.org> ;
    :source <https://github.com/schemaorg/schemaorg/issues/1423> ;
    rdfs:comment "An application programming interface accessible over Web/Internet technologies." ;
    rdfs:subClassOf :Service .
